providers/evercrypt/EverCrypt.Hash.fsti
@@ -229,10 +229,10 @@ val init: #a:e_alg -> (
     footprint s h0 == footprint s h1 /\
     preserves_freeable s h0 h1))
 
-val update_multi_256: Hacl.Hash.Definitions.update_multi_st SHA2_256
+val update_multi_256: Hacl.Hash.Definitions.update_multi_st (|SHA2_256, ()|)
 
 inline_for_extraction noextract
-val update_multi_224: Hacl.Hash.Definitions.update_multi_st SHA2_224
+val update_multi_224: Hacl.Hash.Definitions.update_multi_st (|SHA2_224, ()|)
 
 // Note: this function relies implicitly on the fact that we are running with
 // code/lib/kremlin and that we know that machine integers and secret integers
@@ -282,10 +282,10 @@ val update_multi:
                                                    (B.as_seq h0 blocks)) /\
     preserves_freeable s h0 h1))
 
-val update_last_256: Hacl.Hash.Definitions.update_last_st SHA2_256
+val update_last_256: Hacl.Hash.Definitions.update_last_st (|SHA2_256, ()|)
 
 inline_for_extraction noextract
-val update_last_224: Hacl.Hash.Definitions.update_last_st SHA2_224
+val update_last_224: Hacl.Hash.Definitions.update_last_st (|SHA2_224, ()|)
 
 // 18-03-05 note the *new* length-passing convention!
 // 18-03-03 it is best to let the caller keep track of lengths.
